tests/lean/run/auto_quote1.lean
@@ -1,0 +1,16 @@
+example (a b c : nat) : a = b → b = c → c = a :=
+begin
+  tactic.intros,
+  apply eq.symm,
+  apply eq.trans,
+  assumption,
+  assumption
+end
+
+example (a b c : nat) : a = b → b = c → c = a :=
+begin
+  tactic.intro `h1,
+  tactic.intros,
+  refine eq.symm (eq.trans h1 _),
+  assumption
+end
